\section{Big $\mathcal{O}$ notation}

\begin{definition}
    For $\fnis{f, g} \mathbb{N} \rightarrow \mathbb{R}^{+}$:
    \[ f(n) = \mathcal{O}(g(n)) \defev \exists C > 0, N \in \mathbb{N}: \forall n > N \; f(n) \le C \cdot g(n) \]
    \[ f(n) = \Omega(g(n)) \defev \exists c > 0, N \in \mathbb{N}: \forall n > N \; f(n) \ge c \cdot g(n) \]
    \[ f(n) = \Theta(g(n)) \defev f(n) = \Omega(g(n)) \wedge f(n) = \mathcal{O}(g(n)) \]
\end{definition}

\begin{example}
    Let $T(n) = 2 T(\frac{n}{2}) + \Theta(n)$, then
    \[ T(n) = \Theta(n \log_2{n}) \]
\end{example}
\begin{proof}\phantom\\
\begin{enumerate}
\item
    Prove $T(n) = \mathcal{O}(n \log_2{n})$, i. e. $\exists C > 0 : T(n) \le Cn \log_2{n}$. \\
    \textbf{Base:}
        \[ T(2) \le 2C, T(3) \le C \cdot 3 \log_2{3} \text{ -- true for sufficiently large $C$} \]
    \textbf{Induction step:}
        \[
            T(n) \le
            2 T(\frac{n}{2}) + \mathcal{O}(n) \le
            2 T(\frac{n}{2}) + B n \le
        \]\[
            \le 2 C \frac{n}{2} \log_2{\frac{n}{2}} + Bn =
            C n \log_2{n} + (B - C)n \le C n \log_2{n}
            \text{-- for $C \ge B$}
        \]
\item
    \[ T(n) = \Omega(n \log_2{n}) \]
    By definition, we need to prove $\exists c > 0 : T(n) \le cn \log_2{n}$. \\
    Base: $T(1) \ge c \cdot 0$ -- true \\
    Induction step: $T(n) \ge 2T(\frac{n}{2}) + bn \ge cn \log_2{n} + (b - c) n \ge cn \log_2{n} $ -- for $c \le b$.
\end{enumerate}
\end{proof}

\begin{example}
    Let $T(n) = 2 T\left(\floor{\frac n 2}\right) + \Theta(n)$, then
    \[ T(n) = \mathcal{O}(n \log_2 n) \]
\end{example}
\begin{proof}
    \[ T(n) \le 2C \floor{\frac n 2} \log_2 \floor{\frac n 2} + Bn \le 2C \frac n 2 \log_2 \frac n 2 + Bn = C n \log_2 n + (B - C)n  \]
\end{proof}


\begin{example}
    \[ T(n) = \Omega(n \log_2 n) \]
\end{example}
\begin{proof}
    \[ T(n) \ge 2c \floor{\frac n 2} \log_2 \floor{\frac n 2} + bn \ge 2c \left(\frac n 2 - 1 \right) \log_2 \floor{\frac n 2} + bn = c (n - 2) \log_2 \floor{\frac n 2} + bn \ge (1) \]
    \[ n \ge 2 \implies \floor{\frac n 2} > \frac n 4 \]
    \[ (1) \ge c (n - 2) \log_2 \frac n 4 + bn = c (n - 2) (\log_2 n - 2) + bn = c n \log_2 n + 4c - 2c \log_2 n - 2cn + bn \]
    TODO
\end{proof}

\begin{example}
    Let $T(n) = T\left(\floor{\frac n 2}\right) + T\left(\ceil{\frac n 2}\right) + 1$, then
    \[ T(n) = \Theta(n) \]
\end{example}
\begin{proof}
    Suppose $T(n) \le Cn - D$: \\
    \[ T(n) = T\left(\floor{\frac n 2}\right) + T\left(\ceil{\frac n 2}\right) + 1 \le C \left(\floor{\frac n 2} + \ceil{\frac n 2} \right) - 2D + 1 = Cn - D + (1 - D) \le Cn - D \]

    Suppose $T(n) \ge cn$: \\
    \[ T(n) = T\left(\floor{\frac n 2}\right) + T\left(\ceil{\frac n 2}\right) + 1 \ge c \left(\floor{\frac n 2} + \ceil{\frac n 2} \right) = cn \]
\end{proof}

\begin{example}\textbf{(Guess answer using substitution)} Let $ T(n) = 2 T(\ceil{\sqrt n}) + \log_2 n $, then
    \[ T(n) = \mathcal{O}(\log_2 n \cdot \log_2 \log_2 n) \]
\end{example}
\begin{proof}
    Let $S(x) = T(2 ^ x)$ and ignore ceiling on square root, $S(x) = 2 T(2 ^ {\frac x 2}) + x = 2S(\frac x 2) + x $.
    Then we guess $S(x) = \mathcal{O}(x \log x)$ or $T(n) = \mathcal{O}(\log n \cdot \log \log n)$.

    Suppose $ T(n) \le C \log_2 n \cdot \log_2 \log_2 n $:
    \[
        T(n) =
        2 T(\ceil{\sqrt n}) + \log_2 n \le
        2C \log_2{\ceil{\sqrt n}} \cdot \log_2 \log_2 {\ceil{\sqrt n}} + \log_2 n \le
    \]\[
        \le 2C \log_2{(2 \sqrt n)} \cdot \log_2 \log_2 {\ceil{\sqrt n}} + \log_2 n =
        C \log_2{n} \cdot \log_2 \log_2 {\ceil{\sqrt n}} + 2C\log_2 \log_2 {\ceil{\sqrt n}} + \log_2 n \le
    \]\[
        \le C \log_2{n} \cdot \log_2 \left(\frac 1 2 \log_2 {n} + 1\right) + 2C\log_2 \log_2 {\ceil{\sqrt n}} + \log_2 n \le (\text{for } n \ge 4^{\sqrt{2} + 1})
    \]\[
        \le C \log_2{n} \cdot \log_2 \left(\frac{\log_2 {n}}{\sqrt{2}} \right) + 2C\log_2 \log_2 n + \log_2 n =
    \]\[
        = C \log_2{n} \cdot \log_2 \log_2 {n} + \left( 1 - \frac C 2 \right) \log_2{n} + 2C\log_2 \log_2 n
    \]
    The only thing is left is to kill the last term.
    \[ 2C\log_2 \log_2 {\ceil{\sqrt n}} < \left(\frac C 2 - 1 \right) \log_2{n} \]
\end{proof}

\begin{theorem} (Master theorem)
    $ \fnis{f} \mathbb{N} \rightarrow \mathbb{R^+};\; a, b > 0;\; T(n) = a T(\frac n b) + f(n) $, then
    \begin{itemize}
        \item $f(n) = \mathcal{O}\!\left(n^{\log_b a - \epsilon}\right)$, $\epsilon > 0$: $T(n) = \Theta\left( n^{log_b a} \right)$;
        \item $f(n) = \Theta\!\left(n^{\log_b a}\right)$, $\epsilon > 0$: $T(n) = \Theta\left( n^{\log_b a} \log{n} \right)$;
        \item $f(n) = \Omega\!\left(n^{\log_b a + \epsilon}\right)$, $\epsilon > 0$, $\forall n: a f(\frac{n}{b}) \le c f(n)$, $c < 1$: $T(n) = \Theta(f(n))$.
    \end{itemize}
\end{theorem}

\begin{proof}
Let $a = 1$, $T(n) = T(\floor{\frac n b}) + f(n)$.

\begin{itemize}
    \item $f(n) \le \frac{D}{n^\epsilon}$, then we should prove $T(n) = \Theta(1)$. Suppose $T(n) \le C - \frac E {n^\epsilon}$:
    \[
        T(n) =
        T(\floor{\frac n b}) + f(n) \le
        C - \frac E {\floor{\frac n b}^\epsilon} + \frac{D}{n^\epsilon} \le
        C - \frac E {\left(\frac n b\right)^\epsilon} + \frac{D}{n^\epsilon} =
        C - \frac{E b^\epsilon}{n^\epsilon} + \frac{D}{n^\epsilon} =
        % C - \frac{1}{n^\epsilon} (D - E b^\epsilon}{n^\epsilon}
    \]
    Suppose $T(n) \ge c$:
    \[ T(n) = T(\floor{\frac n b}) + f(n) \ge c + f(n) \ge c \]

    \item $f(n) = \Theta(1)$, then we should prove $T(n) = \Theta(\log n)$. Suppose $T(n) \le C \log_b n$:
    \[
        T(n) =
        T\left(\floor{\frac n b}\right) + f(n) \le
        C \log_b {\frac n b} + D \le C \log_b n - C + D \le C \log_b n
        \text{ -- true if } C > D
    \]
    Suppose $T(n) \ge c \log_b n$:
    \[
        T(n) =
        % T\left(\floor{\frac n b}\right) + f(n) \gt
    \]
    TODO
\end{itemize}

Complete proof left for now.
\end{proof}
